add sub64 to VEX core

Instances/ISAs/VexSummary.lean
@@ -13,6 +13,7 @@ inductive SymExpr (Reg : Type) where
   | low32 : SymExpr Reg → SymExpr Reg
   | uext32 : SymExpr Reg → SymExpr Reg
   | add64 : SymExpr Reg → SymExpr Reg → SymExpr Reg
+  | sub64 : SymExpr Reg → SymExpr Reg → SymExpr Reg
   | load64 : SymMem Reg → SymExpr Reg → SymExpr Reg
   deriving DecidableEq, Repr
 
@@ -124,6 +125,7 @@ mutual
   | .low32 expr => mask32 (evalSymExpr state expr)
   | .uext32 expr => mask32 (evalSymExpr state expr)
   | .add64 lhs rhs => evalSymExpr state lhs + evalSymExpr state rhs
+  | .sub64 lhs rhs => evalSymExpr state lhs - evalSymExpr state rhs
   | .load64 mem addr => ByteMem.read64le (evalSymMem state mem) (evalSymExpr state addr)
 
 @[simp] def evalSymMem {Reg : Type} [DecidableEq Reg] [Fintype Reg]
@@ -155,6 +157,7 @@ def substSymExpr {Reg : Type} [DecidableEq Reg] [Fintype Reg]
   | .low32 expr => .low32 (substSymExpr sub expr)
   | .uext32 expr => .uext32 (substSymExpr sub expr)
   | .add64 lhs rhs => .add64 (substSymExpr sub lhs) (substSymExpr sub rhs)
+  | .sub64 lhs rhs => .sub64 (substSymExpr sub lhs) (substSymExpr sub rhs)
   | .load64 mem addr => .load64 (substSymMem sub mem) (substSymExpr sub addr)
 
 def substSymMem {Reg : Type} [DecidableEq Reg] [Fintype Reg]
@@ -233,6 +236,8 @@ theorem substSymExpr_id {Reg : Type} [DecidableEq Reg] [Fintype Reg] (expr : Sym
   | uext32 expr => simp [substSymExpr, substSymExpr_id]
   | add64 lhs rhs =>
       simp [substSymExpr, substSymExpr_id]
+  | sub64 lhs rhs =>
+      simp [substSymExpr, substSymExpr_id]
   | load64 mem addr =>
       simp [substSymExpr, substSymMem_id, substSymExpr_id]
 
@@ -254,6 +259,8 @@ theorem substSymExpr_compose {Reg : Type} [DecidableEq Reg] [Fintype Reg]
   | low32 expr => simp [substSymExpr, substSymExpr_compose]
   | uext32 expr => simp [substSymExpr, substSymExpr_compose]
   | add64 lhs rhs =>
+      simp [substSymExpr, substSymExpr_compose]
+  | sub64 lhs rhs =>
       simp [substSymExpr, substSymExpr_compose]
   | load64 mem addr =>
       simp [substSymExpr, substSymMem_compose, substSymExpr_compose]
@@ -277,6 +284,8 @@ theorem evalSymExpr_subst {Reg : Type} [DecidableEq Reg] [Fintype Reg]
   | low32 expr => simp [substSymExpr, evalSymExpr_subst]
   | uext32 expr => simp [substSymExpr, evalSymExpr_subst]
   | add64 lhs rhs =>
+      simp [substSymExpr, evalSymExpr_subst]
+  | sub64 lhs rhs =>
       simp [substSymExpr, evalSymExpr_subst]
   | load64 mem addr =>
       simp [substSymExpr, evalSymMem_subst, evalSymExpr_subst]
